theories/ZX/VyZXSPHyperGraph.v
@@ -1,7 +1,7 @@
 Require Export VyZXTensor.
-Require Import SPTensorGraph SPTensorGraphGraph 
+Require Import SPTensorGraph SPTensorGraphGraph
   SPIsomorphismTesting TensorGraph TensorGraphSemantics
-  TensorGraphFacts TensorGraphSP GraphRewriting SPGraphRewriting ZXGraph.
+  TensorGraphFacts TensorGraphSP GraphRewriting SPGraphRewriting SPTensorGraphQuote ZXGraph.
 Require Import VyZXHyperGraph.
 From stdpp Require Import vector pretty.
 
@@ -17,12 +17,12 @@ Fixpoint ZX_spgraph_semantics {n m} (zx : ZX n m) :
   | X n m α => spgraph_of_tensor (Some (true, α)) n m
   | Z n m α => spgraph_of_tensor (Some (false, α)) n m
   | zx0 ↕ zx1 => stack_spgraphs (ZX_spgraph_semantics zx0) (ZX_spgraph_semantics zx1)
-  | zx0 ⟷ zx1 => spcompose_graphs (ZX_spgraph_semantics zx0) (ZX_spgraph_semantics zx1)
+  | zx0 ⟷ zx1 => compose_spgraphs (ZX_spgraph_semantics zx0) (ZX_spgraph_semantics zx1)
   end.
 
 
 Lemma ZX_spgraph_semantics_correct_aux {n m} (zx : ZX n m) :
-  hg_strongperm_eq (cosphg2cohg (ZX_spgraph_semantics zx)) 
+  hg_strongperm_eq (cosphg2cohg (ZX_spgraph_semantics zx))
     (ZX_graph_semantics zx).
 Proof.
   induction zx.
@@ -37,11 +37,11 @@ Proof.
   - cbn.
     now rewrite cosphg2cohg_stack_spgraphs, IHzx1, IHzx2.
   - cbn.
-    now rewrite cosphg2cohg_spcompose_graphs, IHzx1, IHzx2.
+    now rewrite cosphg2cohg_compose_spgraphs, IHzx1, IHzx2.
 Qed.
 
 Lemma ZX_spgraph_semantics_correct {n m} (zx : ZX n m) :
-  graph_semantics (cosphg2cohg (ZX_spgraph_semantics zx)) ≡ 
+  graph_semantics (cosphg2cohg (ZX_spgraph_semantics zx)) ≡
     ZX_tensor_semantics zx.
 Proof.
   rewrite <- ZX_graph_semantics_correct.
@@ -49,7 +49,7 @@ Proof.
 Qed.
 
 Lemma ZX_propeq_of_spgraph_spisomorphic {n m} (zx zx' : ZX n m) :
-  spisomorphic (norm_spverts $ ZX_spgraph_semantics zx) 
+  spisomorphic (norm_spverts $ ZX_spgraph_semantics zx)
     (norm_spverts $ ZX_spgraph_semantics zx') ->
   zx ∝= zx'.
 Proof.
@@ -65,7 +65,25 @@ Proof.
   now apply graph_semantics_isomorphic.
 Qed.
 
-Example spiso_test_example α : 
+Lemma ZX_propeq_of_spgraph_equiv {n m} (zx zx' : ZX n m) :
+   (norm_spverts $ ZX_spgraph_semantics zx) ≡
+    (norm_spverts $ ZX_spgraph_semantics zx') ->
+  zx ∝= zx'.
+Proof.
+  intros (cohg & Hcohg & Hiso)%cosphg2cohg_equiv_gen.
+  unfold proportional_by_1.
+  rewrite <- 2 ZX_tensor_semantics_correct.
+  prep_matrix_equivalence.
+  apply matrix_of_tensor_of_equiv.
+  rewrite <- 2 ZX_spgraph_semantics_correct.
+  rewrite <- 2 (graph_semantics_norm_verts (cosphg2cohg _)).
+  rewrite <- 2 cosphg2cohg_norm_spverts.
+  symmetry.
+  etransitivity; [|apply hg_strongperm_eq_correct; eassumption].
+  now apply graph_semantics_equiv.
+Qed.
+
+Example spiso_test_example α :
   — ↕ Z 1 1 α ⟷ ⊃ ∝= Z 2 0 α.
 Proof.
   apply ZX_propeq_of_spgraph_spisomorphic.
@@ -82,7 +100,7 @@ Ltac spgraph_iso_with n :=
 Ltac zx_ocm_with n :=
   apply ZX_propeq_of_spgraph_spisomorphic;
   spgraph_iso_with n.
-  
+
 
 Ltac zx_ocm :=
   apply ZX_propeq_of_spgraph_spisomorphic;
@@ -90,19 +108,19 @@ Ltac zx_ocm :=
     tryif (
       apply (spgraph_iso_conditions_correct _ _ n);
       vm_compute;
-      lazymatch goal with 
+      lazymatch goal with
       | [|- False] => fail 2 "zx_ocm: No isomorphism found!"
-      | [|- _] => refine ((λ 
+      | [|- _] => refine ((λ
       (_ : (String.concat "" ["Use 'zx_ocm_with "; pretty n; "'"] = "")%string), eq_refl) _);
         vm_compute
       end
-    ) then idtac else go constr:(S n) in 
-  go constr:(O). 
+    ) then idtac else go constr:(S n) in
+  go constr:(O).
 
 
-Example ocm_example : 
+Example ocm_example :
   (Z 1 1 0 ↕ X 1 2 0 ↕ Z 1 1 0) ⟷
-  (X 2 2 0 ↕ X 2 2 0) ⟷ 
+  (X 2 2 0 ↕ X 2 2 0) ⟷
   (Z 1 1 0 ↕ ⊃ ↕ Z 1 1 0) ∝=
   (Z 1 1 0 ↕ (⨉ ⟷ (Z 1 1 0 ↕ X 1 2 0))) ⟷
   (— ↕ ⨉ ↕ —) ⟷
@@ -113,9 +131,9 @@ Proof.
 Qed.
 
 
-Example ocm_example' α β γ : 
+Example ocm_example' α β γ :
   (Z 1 1 γ ↕ X 1 2 α ↕ Z 1 1 β) ⟷
-  (X 2 2 0 ↕ X 2 2 0) ⟷ 
+  (X 2 2 0 ↕ X 2 2 0) ⟷
   (Z 1 1 0 ↕ ⊃ ↕ Z 1 1 0) ∝=
   (Z 1 1 γ ↕ (⨉ ⟷ (Z 1 1 β ↕ X 1 2 α))) ⟷
   (— ↕ ⨉ ↕ —) ⟷
@@ -125,6 +143,81 @@ Proof.
   zx_ocm_with 0.
 Qed.
 
+
+Typeclasses Opaque compose_spgraphs compose_spgraphs_aux stack_spgraphs
+  stack_spgraphs_aux spgraph_of_tensor.
+
+
+Typeclasses Opaque compose_graphs compose_graphs_aux stack_graphs
+  stack_graphs_aux graph_of_tensor.
+
+
+#[export] Hint Extern 0 (CospanSPHyperGraphDenote _ _ (@stack_spgraphs ?T ?n ?m ?n' ?m' ?cohg ?cohg') _) =>
+  notypeclasses refine 
+    (cosphg_denote_stack_spgraphs _ _ (n:=n) (m:=m) (n':=n') (m':=m') 
+      cohg cohg' _ _ _ _) : typeclass_instances.
+#[export] Hint Extern 0 (CospanSPHyperGraphDenote _ _ (@cup_spgraph ?T ?n) _) =>
+  notypeclasses refine 
+    (cosphg_denote_cup_spgraph _ _ (n:=n)) : typeclass_instances.
+#[export] Hint Extern 0 (CospanSPHyperGraphDenote _ _ (@cap_spgraph ?T ?n) _) =>
+  notypeclasses refine 
+    (cosphg_denote_cap_spgraph _ _ (n:=n)) : typeclass_instances.
+#[export] Hint Extern 0 (CospanSPHyperGraphDenote _ _ (@id_spgraph ?T ?n) _) =>
+  notypeclasses refine 
+    (cosphg_denote_id_spgraph _ _ (n:=n)) : typeclass_instances.
+#[export] Hint Extern 0 (CospanSPHyperGraphDenote _ _ (@swap_spgraph ?T ?n ?m) _) =>
+  notypeclasses refine 
+    (cosphg_denote_swap_spgraph _ _ (n:=n) (m:=m)) : typeclass_instances.
+
+#[export] Hint Extern 0 (CospanSPHyperGraphQuote _ _ _ (@stack_spgraphs ?T ?n ?m ?n' ?m' ?cohg ?cohg')) =>
+  notypeclasses refine 
+    (cosphg_quote_stack_spgraphs _ _ (n:=n) (m:=m) (n':=n') (m':=m') 
+      _ _ cohg cohg' _ _) : typeclass_instances.
+#[export] Hint Extern 0 (CospanSPHyperGraphQuote _ _ _ (@cup_spgraph ?T ?n)) =>
+  notypeclasses refine 
+    (cosphg_quote_cup_spgraph _ _ (n:=n)) : typeclass_instances.
+#[export] Hint Extern 0 (CospanSPHyperGraphQuote _ _ _ (@cap_spgraph ?T ?n)) =>
+  notypeclasses refine 
+    (cosphg_quote_cap_spgraph _ _ (n:=n)) : typeclass_instances.
+#[export] Hint Extern 0 (CospanSPHyperGraphQuote _ _ _ (@id_spgraph ?T ?n)) =>
+  notypeclasses refine 
+    (cosphg_quote_id_spgraph _ _ (n:=n)) : typeclass_instances.
+#[export] Hint Extern 0 (CospanSPHyperGraphQuote _ _ _ (@swap_spgraph ?T ?n ?m)) =>
+  notypeclasses refine 
+    (cosphg_quote_swap_spgraph _ _ (n:=n) (m:=m)) : typeclass_instances.
+
+Example ocm_example'_alt γ :
+  (Z 1 (2+2) γ) ⟷ (X 2 2 0 ↕ X 2 2 0) ∝=
+  (Z 1 (2+2) γ) ⟷ (X 2 2 0 ↕ X 2 2 0).
+Proof.
+  apply ZX_propeq_of_spgraph_equiv.
+
+    (* apply spgraph_test_isomorphism_quote. *)
+  unshelve (notypeclasses refine (spgraph_test_isomorphism_quote _ _ _ _ _ _ _ _
+    _ _ _ _); [apply _..|]); [apply nil|].
+  vm_compute.
+  done.
+Qed.
+
+
+Example ocm_example''_alt α β γ :
+  (Z 1 1 γ ↕ X 1 2 α ↕ Z 1 1 β) ⟷
+  (X 2 2 0 ↕ X 2 2 0) ⟷
+  (Z 1 1 0 ↕ ⊃ ↕ Z 1 1 0) ∝=
+  (Z 1 1 γ ↕ (⨉ ⟷ (Z 1 1 β ↕ X 1 2 α))) ⟷
+  (— ↕ ⨉ ↕ —) ⟷
+  (X 2 2 0 ↕ n_wire 2) ⟷
+  (Z 1 1 0 ↕ (X 3 1 0 ⟷ Z 1 1 0)).
+Proof.
+  apply ZX_propeq_of_spgraph_equiv.
+
+    (* apply spgraph_test_isomorphism_quote. *)
+  unshelve (notypeclasses refine (spgraph_test_isomorphism_quote _ _ _ _ _ _ _ _
+    _ _ _ _); [cbn; apply _..|]); [apply nil|];
+  vm_compute.
+  done.
+Qed.
+
 (* Fixpoint example_Z_stack_prf (n : nat) : S n = n + 1 :=
   match n with
   | O => eq_refl
@@ -132,23 +225,89 @@ Qed.
   end.
 
 Fixpoint example_Z_stack (n : nat) : ZX n n :=
-  match n with 
+  match n with
   | O => ⦰
   | S n' => cast _ _ (example_Z_stack_prf n') (example_Z_stack_prf n')
     $ example_Z_stack n' ↕ Z 1 1 (INR n')
   end.
 
 Fixpoint example_Z_stack_rev (n : nat) : ZX n n :=
-  match n with 
+  match n with
   | O => ⦰
   | S n' => Z 1 1 (INR n') ↕ example_Z_stack_rev n'
   end.
 
-Example ocm_example'' : forall n, 
+Section alt.
+
+Context `{Equiv T, !RelDecision (≡@{T})}.
+Fixpoint sphyperedge_map_isos_extending_aux' 
+  (hg hg' : list (positive * (T * list (positive * positive))))
+  (mhe_mv : Piso * Piso) :
+  list (Piso * Piso) :=
+  match hg with
+  | [] => match hg' with | [] => [mhe_mv] | _::_ => [] end
+  | (k, (t, v)) :: hg =>
+    list_select (λ k_tv, t ≡ k_tv.2.1 /\ 
+      sum_list_with Pos.to_nat (k_tv.2.2).*2 = 
+      sum_list_with Pos.to_nat v.*2) hg'
+      ≫= λ '(k_tv, hg'rest),
+      match pupdate k k_tv.1 mhe_mv.1 with
+      | None => []
+      | Some mhe' =>
+        mv' ← gmultiset_pre_isos_extending_aux_alt v k_tv.2.2 mhe_mv.2;
+        sphyperedge_map_isos_extending_aux' hg hg'rest
+         (mhe', mv')
+      end
+  end.
+
+Import Datatypes.
+
+Definition sphyperedge_map_isos_extending'
+  (hg hg' : Pmap (SPHyperEdge T)) (mhe_mv : Piso * Piso) :
+  list (Piso * Piso) :=
+  sphyperedge_map_isos_extending_aux' 
+    (prod_map id (prod_map id (map_to_list (M:=gmap positive positive) ∘ gmultiset_car)) <$> 
+      (map_to_list hg :> list (positive * (T * gmultiset positive))))
+    (prod_map id (prod_map id (map_to_list (M:=gmap positive positive) ∘ gmultiset_car)) <$> 
+      (map_to_list hg' :> list (positive * (T * gmultiset positive))))
+    mhe_mv.
+
+Definition spgraph_isos' {n m} (cohg cohg' : CospanSPHyperGraph T n m) :
+  list (Piso * Piso) :=
+  if decide (size (spisolated_vertices cohg) = size (spisolated_vertices cohg')) then
+    default []
+      (mv ← pupdates (zip (cohg.(spinputs) ++ cohg.(spoutputs))
+        (cohg'.(spinputs) ++ cohg'.(spoutputs))) ∅;
+      Some
+      (sphyperedge_map_isos_extending' cohg.(sphedges).(sphyperedges)
+        cohg'.(sphedges).(sphyperedges) (∅, mv)))
+  else
+    [].
+
+End alt.
+
+Example ocm_example'' : forall n,
   Z 1 n 0 ⟷ example_Z_stack n ⟷ Z n 1 0 ∝=
   Z 1 n 0 ⟷ example_Z_stack_rev n ⟷ Z n 1 0.
 Proof.
   intros n.
-  assert (n = 5) by admit.
+  assert (n = 7) by admit.
   subst.
+  
+  apply ZX_propeq_of_spgraph_equiv.
+
+    (* apply spgraph_test_isomorphism_quote. *)
+  Time unshelve (notypeclasses refine (spgraph_test_isomorphism_quote _ _ _ _ _ _ _ _
+    _ _ _ _); [cbn; apply _..|]); [apply nil|];
+  remember (@spgraph_iso_partial_test _ _ _) as f eqn:Hf;
+  vm_compute;
+  subst f.
+  unfold spgraph_iso_partial_test.
+  replace @spgraph_isos with @spgraph_isos' by admit.
+  Time vm_compute.
+  replace @spgraph_isos with @spgraph_isos' by admit.
+
+  vm_compute.
+  done.
+Qed.
   Time zx_ocm. *)
