theories/GraphCore/IsomorphismTestingAux.v
@@ -1,0 +1,862 @@
+From stdpp Require Export pmap. 
+Require Export Aux_pos Aux_relset.
+
+
+Lemma list_filter_bind {A B} {P : B -> Prop} `{forall b, Decision (P b)}
+  (f : A -> list B) (l : list A) :
+  filter P (l ≫= f) = l ≫= filter P ∘ f.
+Proof.
+  induction l; [done|].
+  cbn.
+  now rewrite filter_app; f_equal.
+Qed.
+
+Lemma list_bind_filter {A B} {P : A -> Prop} `{forall b, Decision (P b)}
+  (f : A -> list B) (l : list A) :
+  filter P l ≫= f = l ≫= λ a, if decide (P a) then f a else [].
+Proof.
+  induction l; [done|].
+  cbn.
+  case_decide; cbn; [f_equal|]; apply IHl.
+Qed.
+
+Lemma list_filter_to_bind {A} (P : A -> Prop) `{forall a, Decision (P a)}
+  (l : list A) : filter P l = l ≫= λ x, filter P [x].
+Proof.
+  cbn.
+  induction l; [done|].
+  cbn.
+  case_decide; cbn; f_equal; apply IHl.
+Qed.
+
+Lemma list_select_and {A} (P Q : A -> Prop) `{forall a, Decision (P a)}
+  `{forall a, Decision (Q a)} (l : list A) :
+  list_select (λ a, P a /\ Q a) l = filter (λ a_as, P a_as.1) $ list_select Q l.
+Proof.
+  unfold list_select.
+  rewrite list_filter_filter.
+  done.
+Qed.
+
+
+Lemma map_inverses_inj_l `{FinMap K1 M1, FinMap K2 M2}
+  (m1 m1' : M1 K2) (m2 : M2 K1) :
+  map_inverses m1 m2 -> map_inverses m1' m2 ->
+  m1 = m1'.
+Proof.
+  intros Hinv Hinv'.
+  apply map_eq.
+  intros k.
+  apply option_eq; intros x.
+  now rewrite (Hinv k x), (Hinv' k x).
+Qed.
+
+Lemma map_inverses_inj_r `{FinMap K1 M1, FinMap K2 M2}
+  (m1 : M1 K2) (m2 m2' : M2 K1) :
+  map_inverses m1 m2 -> map_inverses m1 m2' ->
+  m2 = m2'.
+Proof.
+  intros Hinv Hinv'.
+  apply map_eq.
+  intros k.
+  apply option_eq; intros x.
+  now rewrite <- (Hinv x k), <- (Hinv' x k).
+Qed.
+
+Lemma map_inverses_delete_Some `{FinMap K1 M1, FinMap K2 M2}
+  (m1 : M1 K2) (m2 : M2 K1) k1 k2 :
+  map_inverses m1 m2 -> m1 !! k1 = Some k2 ->
+  map_inverses (delete k1 m1) (delete k2 m2).
+Proof.
+  intros Hinv Hmk1 k1' k2'.
+  destruct_decide (decide (k1' = k1)) as Hk1.
+  - subst k1'.
+    rewrite lookup_delete.
+    split; [easy|].
+    intros (Hk2 & Heq)%lookup_delete_Some.
+    contradict Hk2.
+    rewrite <- (Hinv _ _) in Heq.
+    congruence.
+  - rewrite lookup_delete_ne by done.
+    rewrite (Hinv _ _).
+    split; [|now intros []%lookup_delete_Some].
+    intros Hlook.
+    rewrite (Hinv _ _) in Hmk1.
+    now rewrite lookup_delete_ne by congruence.
+Qed.
+
+
+Lemma map_inverses_delete_None `{FinMap K1 M1, FinMap K2 M2}
+  (m1 : M1 K2) (m2 : M2 K1) k1 :
+  map_inverses m1 m2 -> m1 !! k1 = None ->
+  map_inverses (delete k1 m1) m2.
+Proof.
+  intros Hinv Hmk1.
+  now rewrite delete_notin by done.
+Qed.
+
+Lemma map_inverses_delete_case `{FinMap K1 M1, FinMap K2 M2}
+  (m1 : M1 K2) (m2 : M2 K1) k1 :
+  map_inverses m1 m2 ->
+  map_inverses (delete k1 m1) (match m1 !! k1 with
+    | None => m2
+    | Some k2 => delete k2 m2
+    end).
+Proof.
+  intros Hinv.
+  case_match eqn:Heq.
+  - now apply map_inverses_delete_Some.
+  - now apply map_inverses_delete_None.
+Qed.
+
+Lemma map_inverses_iff_perm `{FinMap K1 M1, FinMap K2 M2}
+  (m1 : M1 K2) (m2 : M2 K1) : map_inverses m1 m2 <->
+  map_to_list m1 ≡ₚ prod_swap <$> map_to_list m2.
+Proof.
+  split.
+  - intros Hinv.
+    apply NoDup_Permutation; [apply NoDup_map_to_list|
+      apply (NoDup_fmap _), NoDup_map_to_list|..].
+    intros (k1 & k2).
+    rewrite elem_of_map_to_list.
+    change (k1, k2) with (prod_swap (k2, k1)).
+    rewrite (elem_of_list_fmap_inj _).
+    rewrite elem_of_map_to_list.
+    apply Hinv.
+  - intros Heq k1 k2.
+    rewrite <- 2 elem_of_map_to_list.
+    rewrite Heq.
+    change (k1, k2) with (prod_swap (k2, k1)).
+    apply (elem_of_list_fmap_inj _).
+Qed.
+
+#[export] Instance map_inverses_dec `{FinMap K1 M1, FinMap K2 M2}
+  (m1 : M1 K2) (m2 : M2 K1) : Decision (map_inverses m1 m2).
+  refine (cast_if (decide (map_to_list m1 ≡ₚ prod_swap <$> map_to_list m2))).
+  abstract (now rewrite map_inverses_iff_perm).
+  abstract (now rewrite map_inverses_iff_perm).
+Defined.
+
+Record Piso := mk_Piso' {
+  Piso_map : Pmap positive;
+  Piso_invmap : Pmap positive;
+  Piso_inverses' : Is_true (bool_decide (map_inverses Piso_map Piso_invmap));
+}.
+
+#[global] Coercion Piso_map : Piso >-> Pmap.
+
+#[export] Instance Piso_equiv : Equiv Piso :=
+  fun m m' => m.(Piso_map) = m'.(Piso_map) /\
+    m.(Piso_invmap) = m'.(Piso_invmap).
+
+#[export] Instance Piso_equivalence : @Equivalence Piso equiv.
+Proof.
+  apply rel_intersection_equiv; refine (rel_preimage_equiv _ _ _).
+Qed.
+
+#[export] Instance Piso_leibniz : LeibnizEquiv Piso.
+Proof.
+  intros [m mi Hmi] [m' mi' Hmi'] [[= <-] [= <-]].
+  f_equal.
+  apply proof_irrel.
+Qed.
+
+Lemma Piso_inverses m : map_inverses m.(Piso_map) m.(Piso_invmap).
+Proof.
+  refine (bool_decide_unpack _ _).
+  apply Piso_inverses'.
+Qed.
+
+Definition mk_Piso (m mi : Pmap positive) (Hmmi : map_inverses m mi) : Piso :=
+  mk_Piso' m mi (bool_decide_pack _ Hmmi).
+
+
+Lemma Piso_equiv_iff (m m' : Piso) : m ≡ m' <->
+  m.(Piso_map) = m'.(Piso_map).
+Proof.
+  split; [now intros []|].
+  intros Hmap.
+  split; [done|].
+  apply map_inverses_inj_r with m.(Piso_map).
+  - apply Piso_inverses.
+  - rewrite Hmap.
+    apply Piso_inverses.
+Qed.
+
+
+#[export] Instance Piso_empty : Empty Piso :=
+  mk_Piso ∅ ∅ map_inverses_empty.
+
+Definition Piso_inverse (m : Piso) : Piso :=
+  mk_Piso m.(Piso_invmap) m.(Piso_map)
+    ((map_inverses_comm _ _).1 (Piso_inverses m)).
+
+Add Parametric Morphism : Piso_inverse with signature equiv ==> equiv
+  as Piso_inverse_proper.
+Proof.
+  now intros ? ? [].
+Qed.
+
+#[export] Instance Piso_delete : Delete positive Piso :=
+  fun k m =>
+  mk_Piso (delete k m.(Piso_map)) _
+    (map_inverses_delete_case _ _ k (Piso_inverses m)).
+
+Add Parametric Morphism : (@delete positive Piso _) with signature
+  eq ==> equiv ==> equiv as Piso_delete_proper.
+Proof.
+  intros k m m' [Hm Hmi].
+  split; [now unfold delete; cbn; f_equal|].
+  unfold delete; cbn.
+  rewrite <- Hm.
+  case_match; [f_equal|]; apply Hmi.
+Qed.
+
+
+Definition pinsert (k v : positive) (m : Piso) : option Piso :=
+  match m.(Piso_map) !! k as mk
+    return (mk = None -> _) -> _ with
+  | Some _ => fun _ => None
+  | None => fun H =>
+    match m.(Piso_invmap) !! v as mv return (mv = None -> _) -> _ with
+    | Some _ => fun _ => None
+    | None => fun H =>
+  Some (mk_Piso (insert k v m.(Piso_map))
+    (insert v k m.(Piso_invmap)) (H eq_refl))
+    end (H eq_refl)
+  end
+    (map_inverses_insert_fresh m.(Piso_map) m.(Piso_invmap) k v (Piso_inverses m)).
+
+
+(* Definition pinsert (k v : positive) (m : Piso) : option Piso :=
+  match m.(Piso_map) !! k as mk, m.(Piso_invmap) !! v as mv
+    return (mk = None -> mv = None -> _) -> _ with
+  | None, None => fun H =>
+    Some (mk_Piso (insert k v m.(Piso_map))
+      (insert v k m.(Piso_invmap)) (H eq_refl eq_refl))
+  | _, _ => fun _ => None
+  end
+    (map_inverses_insert_fresh m.(Piso_map) m.(Piso_invmap) k v m.(Piso_inverses)). *)
+
+Lemma pinsert_correct k v (m : Piso) m' :
+  pinsert k v m = Some m' ->
+  m'.(Piso_map) = <[k := v]> m.(Piso_map).
+Proof.
+  unfold pinsert.
+  generalize (map_inverses_insert_fresh m.(Piso_map) m.(Piso_invmap) k v (Piso_inverses m)).
+  do 2 (case_match; [done|]).
+  intros ? [= <-].
+  done.
+Qed.
+
+Definition pupdate k v (m : Piso) : option Piso :=
+  match (m :> Pmap _) !! k with
+  | None => pinsert k v m
+  | Some v' => if decide (v = v') then Some m else None
+  end.
+
+Lemma pupdate_correct k v m m' : pupdate k v m = Some m' ->
+  m'.(Piso_map) !! k = Some v.
+Proof.
+  unfold pupdate.
+  case_match eqn:Hmk; [now case_decide; congruence|].
+  intros ->%pinsert_correct.
+  apply lookup_insert.
+Qed.
+
+(* Fixpoint pinserts (kvs : list (positive * positive)) (m : Piso) : option Piso :=
+  match kvs with
+  | [] => Some m
+  | (k, v) :: kvs =>
+    pinsert k v m ≫= pinserts kvs
+  end.
+
+Lemma pinserts_correct kvs m m' :
+  pinserts kvs m = Some m' ->
+  list_to_map kvs ∪ m.(Piso_map) ⊆@{Pmap _} m' /\
+  list_to_set kvs.*1 ## dom m.(Piso_map) /\
+  NoDup kvs.*1 /\ NoDup kvs.*2.
+Proof.
+  revert m m'; induction kvs as [|[k v] kvs IHkvs];
+  intros m m'; [intros [= <-]; cbn; now rewrite (map_empty_union _)|].
+  cbn.
+  intros (m'' & Heq%pinsert_correct & <-%IHkvs)%bind_Some.
+  rewrite Heq.
+
+  pose proof Heq as Heq'.
+  pose proof Hkvs as Hkvs'.
+
+  etransitivity
+  rewrite Hkvs. *)
+
+
+Fixpoint pupdates (kvs : list (positive * positive)) (m : Piso) : option Piso :=
+  match kvs with
+  | [] => Some m
+  | (k, v) :: kvs =>
+    pupdates kvs m ≫= pupdate k v
+  end.
+
+Lemma pupdate_correct_subseteq k v m m' :
+  pupdate k v m = Some m' ->
+  <[k := v]> m.(Piso_map) ⊆ m'.(Piso_map).
+Proof.
+  unfold pupdate.
+  case_match; [|now intros ->%pinsert_correct].
+  case_decide; [|done].
+  intros [= <-].
+  subst.
+  now apply eq_reflexivity, insert_id.
+Qed.
+
+Lemma pupdates_correct_subseteq kvs m m' :
+  pupdates kvs m = Some m' ->
+  list_to_map kvs ∪ m.(Piso_map) ⊆@{Pmap _} m'.
+Proof.
+  revert m m'; induction kvs as [|[k v] kvs IHkvs];
+  intros m m'; [intros [= <-]; cbn; now rewrite (map_empty_union _)|].
+  cbn.
+  intros (m'' & Heq & Hkvs)%bind_Some.
+  apply pupdate_correct_subseteq in Hkvs as Hkvs'.
+  rewrite <- Hkvs', <- insert_union_l.
+  apply insert_mono.
+  now apply IHkvs.
+Qed.
+
+Lemma pupdate_correct_extends k v m m' :
+  pupdate k v m = Some m' ->
+  m.(Piso_map) ⊆ m'.(Piso_map).
+Proof.
+  unfold pupdate.
+  case_match eqn:Hmk; [|intros ->%pinsert_correct; now apply insert_subseteq].
+  case_decide; [|done].
+  now intros [= <-].
+Qed.
+
+Lemma pupdates_correct_extends kvs m m' :
+  pupdates kvs m = Some m' ->
+  m.(Piso_map) ⊆@{Pmap _} m'.
+Proof.
+  revert m m'; induction kvs as [|[k v] kvs IHkvs];
+  intros m m'; [now intros [= <-]|].
+  cbn.
+  intros (m'' & Heq & Hkvs)%bind_Some.
+  apply pupdate_correct_extends in Hkvs as Hkvs'.
+  rewrite <- Hkvs'.
+  now apply IHkvs in Heq.
+Qed.
+
+Lemma pupdates_correct kvs m m' :
+  pupdates kvs m = Some m' ->
+  Forall (λ '(k, v), m'.(Piso_map) !! k = Some v) kvs.
+Proof.
+  revert m m'; induction kvs as [|[k v] kvs IHkvs];
+  intros m m'; [done|].
+  intros Heq.
+  constructor.
+  - apply pupdates_correct_subseteq in Heq.
+    cbn in Heq.
+    revert Heq.
+    apply lookup_weaken.
+    rewrite <- insert_union_l.
+    apply lookup_insert.
+  - cbn in Heq.
+    apply bind_Some in Heq as (m'' & Hkvs & Heq).
+    apply IHkvs in Hkvs as Hall.
+    eapply Forall_impl; [apply Hall|].
+    intros (k', v') Hlook.
+    apply pupdate_correct_extends in Heq.
+    revert Heq.
+    now apply lookup_weaken.
+Qed.
+
+Lemma pinsert_spec_1 k v m m' :
+  pinsert k v m = Some m' -> m'.(Piso_map) = <[k := v]> m.(Piso_map) /\
+    m'.(Piso_invmap) = <[v := k]> m.(Piso_invmap) /\
+    (Piso_map m) !! k = None /\ (Piso_invmap m) !! v = None.
+Proof.
+  unfold pinsert.
+  remember (map_inverses_insert_fresh _ _ _ _ _) as Hprf eqn:Hprfeq.
+  clear Hprfeq.
+  case_match; [done|].
+  case_match; [done|].
+  intros [= <-].
+  done.
+Qed.
+
+Lemma pinsert_spec k v m m' :
+  pinsert k v m = Some m' <-> m'.(Piso_map) = <[k := v]> m.(Piso_map) /\
+    (Piso_map m) !! k = None /\ (Piso_invmap m) !! v = None.
+Proof.
+  split.
+  - unfold pinsert.
+    remember (map_inverses_insert_fresh _ _ _ _ _) as Hprf eqn:Hprfeq.
+    clear Hprfeq.
+    case_match; [done|].
+    case_match; [done|].
+    intros [= <-].
+    done.
+  - unfold pinsert.
+    remember (map_inverses_insert_fresh _ _ _ _ _) as Hprf eqn:Hprfeq.
+    clear Hprfeq.
+    intros (Hm' & Hmk & Hmik).
+    case_match; [done|].
+    case_match; [done|].
+    f_equal.
+    apply leibniz_equiv_iff, Piso_equiv_iff.
+    now cbn.
+Qed.
+
+Lemma pinsert_is_Some k v m :
+  is_Some (pinsert k v m) <-> m.(Piso_map) !! k = None /\ m.(Piso_invmap) !! v = None.
+Proof.
+  split; [now intros [? ?%pinsert_spec]|].
+  intros [Hm Hmi].
+  unfold pinsert.
+  remember (map_inverses_insert_fresh _ _ _ _ _) as Hprf eqn:Hprfeq.
+  clear Hprfeq.
+  case_match; [done|].
+  case_match; [done|].
+  trivial.
+Qed.
+
+Lemma pupdate_correct_insert k v m m' : 
+  pupdate k v m = Some m' -> m'.(Piso_map) = <[k := v]> m.(Piso_map).
+Proof.
+  unfold pupdate.
+  destruct (m.(Piso_map) !! k) as [mk|] eqn:Hmk.
+  - case_decide; [subst|done].
+    intros [= <-].
+    symmetry.
+    now apply insert_id.
+  - apply pinsert_correct.
+Qed.
+
+Lemma Piso_invmap_subseteq m m' :
+  Piso_map m ⊆ Piso_map m' -> Piso_invmap m ⊆ Piso_invmap m'.
+Proof.
+  intros Hsubs.
+  rewrite map_subseteq_spec in *.
+  intros k v.
+  rewrite <- 2 (Piso_inverses _ _ _).
+  apply Hsubs.
+Qed.
+
+Lemma pinsert_comm_bind k1 v1 k2 v2 m :
+  pinsert k1 v1 m ≫= pinsert k2 v2 = pinsert k2 v2 m ≫= pinsert k1 v1.
+Proof.
+  apply option_eq; intros m2.
+  rewrite 2 bind_Some.
+  split.
+  - intros (m1 & (Heq & Heqi & Hmk1 & Hmiv1)%pinsert_spec_1 &
+      (Heq' & Heqi' & Hm1k2 & Hmi1v2)%pinsert_spec_1).
+    assert (Hins : is_Some (pinsert k2 v2 m)). 1:{
+      apply pinsert_is_Some.
+      rewrite Heq in Hm1k2.
+      apply lookup_insert_None in Hm1k2.
+      split; [apply Hm1k2|].
+      rewrite Heqi in Hmi1v2.
+      apply lookup_insert_None in Hmi1v2.
+      apply Hmi1v2.
+    }
+    destruct Hins as (m3 & Hm3ins).
+    pose proof Hm3ins as (Hm3 & Hmi3 & Hmk2 & Hmiv2)%pinsert_spec_1.
+    exists m3.
+    split; [done|].
+    apply pinsert_spec.
+    assert (Hk1k2 : k1 <> k2) by now rewrite Heq, lookup_insert_None in Hm1k2.
+    assert (Hv1v2 : v1 <> v2) by now rewrite Heqi, lookup_insert_None in Hmi1v2.
+    rewrite Hm3.
+    rewrite lookup_insert_ne by done.
+    rewrite Hmi3.
+    rewrite lookup_insert_ne by done.
+    split; [|done].
+    rewrite Heq', Heq.
+    now apply insert_commute.
+  - intros (m1 & (Heq & Heqi & Hmk1 & Hmiv1)%pinsert_spec_1 &
+      (Heq' & Heqi' & Hm1k2 & Hmi1v2)%pinsert_spec_1).
+    assert (Hins : is_Some (pinsert k1 v1 m)). 1:{
+      apply pinsert_is_Some.
+      rewrite Heq in Hm1k2.
+      apply lookup_insert_None in Hm1k2.
+      split; [apply Hm1k2|].
+      rewrite Heqi in Hmi1v2.
+      apply lookup_insert_None in Hmi1v2.
+      apply Hmi1v2.
+    }
+    destruct Hins as (m3 & Hm3ins).
+    pose proof Hm3ins as (Hm3 & Hmi3 & Hmk2 & Hmiv2)%pinsert_spec_1.
+    exists m3.
+    split; [done|].
+    apply pinsert_spec.
+    assert (Hk1k2 : k1 <> k2) by now rewrite Heq, lookup_insert_None in Hm1k2.
+    assert (Hv1v2 : v1 <> v2) by now rewrite Heqi, lookup_insert_None in Hmi1v2.
+    rewrite Hm3.
+    rewrite lookup_insert_ne by done.
+    rewrite Hmi3.
+    rewrite lookup_insert_ne by done.
+    split; [|done].
+    rewrite Heq', Heq.
+    now apply insert_commute.
+Qed.
+
+Lemma pupdates_perm kvs kvs' m m' :
+  kvs ≡ₚ kvs' -> pupdates kvs m = Some m' -> pupdates kvs' m = Some m'.
+Proof.
+  intros Hkvs.
+  revert m m'.
+  induction Hkvs; intros m m'.
+  - done.
+  - cbn.
+    case_match; subst.
+    intros (m'' & Hkvs' & Heq)%bind_Some.
+    apply IHHkvs in Hkvs'.
+    rewrite Hkvs'.
+    now cbn.
+  - cbn.
+    destruct x as [k1 v1], y as [k2 v2].
+    cbn.
+    destruct (pupdates l m) as [m''|]; [|done].
+    cbn.
+    unfold pupdate at 2.
+    case_match eqn:Hm''k1. 1:{
+      case_decide; [|done].
+      cbn.
+      subst.
+      intros Heq.
+      rewrite Heq.
+      cbn.
+      apply pupdate_correct_extends in Heq as Heq'.
+      unfold pupdate.
+      eapply lookup_weaken in Hm''k1 as Hm'k1; [|eassumption].
+      rewrite Hm'k1.
+      now apply decide_True.
+    }
+    intros (m1 & Hm1 & Hupd)%bind_Some.
+    revert Hupd.
+    unfold pupdate at 1.
+    apply pinsert_correct in Hm1 as Hm1eq.
+    rewrite Hm1eq.
+    rewrite lookup_insert_case.
+    case_decide as Hk1k2. 1:{
+      case_decide; [|done].
+      intros [= <-].
+      subst.
+      unfold pupdate at 2.
+      rewrite Hm''k1, Hm1.
+      cbn.
+      unfold pupdate.
+      rewrite Hm1eq, lookup_insert.
+      now apply decide_True.
+    }
+    case_match eqn:Hm''k2. 1:{
+      case_decide; [|done].
+      subst.
+      intros [= <-].
+      unfold pupdate at 2.
+      rewrite Hm''k2.
+      rewrite decide_True by done.
+      cbn.
+      unfold pupdate.
+      rewrite Hm''k1.
+      done.
+    }
+    intros Hm2.
+    unfold pupdate at 2.
+    rewrite Hm''k2.
+    replace (Some m') with (pinsert k2 v2 m'' ≫= pinsert k1 v1);
+    [|rewrite pinsert_comm_bind, Hm1; apply Hm2].
+    destruct (pinsert k2 v2 m'') as [m3|] eqn:Hm3; [|done].
+    cbn.
+    unfold pupdate.
+    apply pinsert_spec_1 in Hm3.
+    rewrite Hm3.1.
+    rewrite lookup_insert_ne by done.
+    now rewrite Hm''k1.
+  - eauto.
+Qed.
+
+
+Lemma list_bind_mono_l {A B} (f : A -> list B) (l l' : list A) :
+  l ⊆ l' ->
+  l ≫= f ⊆ l' ≫= f.
+Proof.
+  intros Hl.
+  intros x.
+  rewrite 2 elem_of_list_bind.
+  naive_solver.
+Qed.
+
+Lemma list_bind_mono_r {A B} (f g : A -> list B) (l : list A) :
+  (forall x, x ∈ l -> f x ⊆ g x) ->
+  l ≫= f ⊆ l ≫= g.
+Proof.
+  rewrite <- Forall_forall.
+  intros Hl.
+  induction Hl; [done|cbn].
+  now apply list_subseteq_app.
+Qed.
+
+Lemma list_bind_mono {A B} (f g : A -> list B) (l l' : list A) :
+  (forall x, x ∈ l -> f x ⊆ g x) ->
+  l ⊆ l' ->
+  l ≫= f ⊆ l' ≫= g.
+Proof.
+  intros ->%list_bind_mono_r.
+  apply list_bind_mono_l.
+Qed.
+
+
+Definition extend_posmap_one k v (m : Pmap positive) : option (Pmap positive) :=
+  match m !! k with
+  | None => Some (<[k := v]> m)
+  | Some v' =>
+    if decide (v = v') then
+      Some m
+    else
+      None
+  end.
+
+Lemma extend_posmap_one_Some k v m m' :
+  extend_posmap_one k v m = Some m' ->
+  m ⊆ m' /\
+  m' !! k = Some v /\
+  dom m' = dom m ∪ {[k]}.
+Proof.
+  unfold extend_posmap_one.
+  destruct (m !! k) as [mk|] eqn:Hmk.
+  - case_decide as Heq; [|done].
+    intros [= <-].
+    subst mk.
+    split; [done|].
+    split; [done|].
+    apply elem_of_dom_2 in Hmk.
+    set_solver.
+  - intros [= <-].
+    split; [now apply insert_subseteq|].
+    split; [now rewrite lookup_insert|].
+    rewrite dom_insert_L.
+    apply union_comm_L.
+Qed.
+
+
+Fixpoint extend_posmap (l : list (positive * positive))
+  (m : Pmap positive) : option (Pmap positive) :=
+  match l with
+  | [] => Some m
+  | kv :: l =>
+    match m !! kv.1 with
+    | None => extend_posmap l (<[kv.1 := kv.2]> m)
+    | Some v' =>
+      if decide (kv.2 = v') then
+        extend_posmap l m
+      else
+        None
+    end
+  end.
+
+Lemma extend_posmap_cons k v l m :
+  extend_posmap ((k, v) :: l) m =
+  extend_posmap_one k v m ≫= extend_posmap l.
+Proof.
+  cbn.
+  unfold extend_posmap_one.
+  now case_match; [case_decide|].
+Qed.
+
+Lemma extend_posmap_Some l m m' :
+  extend_posmap l m = Some m' ->
+  m ⊆ m' /\
+  Forall (λ kv, m' !! kv.1 = Some kv.2) l /\
+  dom m' = dom m ∪ list_to_set l.*1 /\
+  map_img m' =@{Pset} map_img m ∪ list_to_set l.*2.
+Proof.
+  revert m; induction l as [|(k,v) l IHl]; intros m.
+  - cbn.
+    intros [= <-].
+    split; [done|].
+    split; [constructor|].
+    now rewrite 2 union_empty_r_L.
+  - cbn -[union].
+    destruct (m !! k) as [mk|] eqn:Hmk.
+    + case_decide as Hvk; [|done].
+      subst mk.
+      intros (Hm & Hall & Hdom & Himg)%IHl.
+      split; [done|].
+      split; [constructor; [|done];
+        revert Hm; now apply lookup_weaken|].
+      rewrite Hdom, Himg.
+      rewrite 2 union_assoc_L.
+      split; f_equal;
+      [apply elem_of_dom_2 in Hmk|
+      apply (elem_of_map_img_2 (SA:=Pset)) in Hmk];
+      set_solver +Hmk.
+    + intros (Hm & Hall & Hdom & Himg)%IHl.
+      split; [rewrite <- Hm; now apply insert_subseteq|].
+      split; [|split; [apply leibniz_equiv_iff; rewrite Hdom, dom_insert;
+        intros x; rewrite 4 elem_of_union; tauto|
+        apply leibniz_equiv_iff; rewrite Himg, map_img_insert,
+          delete_notin by done; intros x; rewrite 4 elem_of_union; tauto]].
+      constructor; [|done].
+      cbn.
+      revert Hm.
+      apply lookup_weaken, lookup_insert.
+Qed.
+
+
+Lemma extend_posmap_Some' l m m' :
+  extend_posmap l m = Some m' ->
+  m ⊆ m' /\
+  Forall2 (λ k v, m' !! k = Some v) l.*1 l.*2 /\
+  dom m' = dom m ∪ list_to_set l.*1.
+Proof.
+  intros (Hm & Hall & Hdom & Himg)%extend_posmap_Some.
+  split; [done|].
+  split; [|done].
+  rewrite Forall2_lookup.
+  rewrite Forall_lookup in Hall.
+  intros i.
+  rewrite 2 list_lookup_fmap.
+  destruct (l !! i) as [li|] eqn:Hli; [|constructor].
+  cbn.
+  constructor.
+  now apply (Hall i).
+Qed.
+
+
+Lemma extend_posmap_Some_fmap l m m' :
+  extend_posmap l m = Some m' ->
+  (m' !!.) <$> l.*1 = Some <$> l.*2.
+Proof.
+  intros (Hm & Heq & Hdom)%extend_posmap_Some.
+  rewrite <- 2 list_fmap_compose.
+  apply list_fmap_ext.
+  intros _ (k, v) Hkv%elem_of_list_lookup_2.
+  rewrite Forall_forall in Heq.
+  now apply Heq in Hkv.
+Qed.
+
+Lemma extend_posmap_app l l' m :
+  extend_posmap (l ++ l') m =
+  extend_posmap l m ≫= extend_posmap l'.
+Proof.
+  revert m; induction l as [|(k, v) l IHl]; intros m; [done|].
+  cbn -[extend_posmap].
+  rewrite 2 extend_posmap_cons.
+  destruct (extend_posmap_one _ _ _); [|done].
+  cbn.
+  apply IHl.
+Qed.
+
+Lemma extend_posmap_one_Piso_map k v m m' :
+  pinsert k v m = Some m' ->
+  extend_posmap_one k v m.(Piso_map) = Some m'.(Piso_map).
+Proof.
+  intros Heq.
+  apply pinsert_spec in Heq.
+  unfold extend_posmap_one.
+  rewrite Heq.2.1, Heq.1.
+  done.
+Qed.
+
+
+Lemma extend_posmap_one_Piso_map' k v m m' :
+  pupdate k v m = Some m' ->
+  extend_posmap_one k v m.(Piso_map) = Some m'.(Piso_map).
+Proof.
+  unfold pupdate.
+  case_match eqn:Hmk; [|apply extend_posmap_one_Piso_map].
+  case_decide; [|done].
+  subst.
+  intros [= <-].
+  unfold extend_posmap_one.
+  rewrite Hmk.
+  now apply decide_True.
+Qed.
+
+Lemma pupdates_app kvs kvs' m :
+  pupdates (kvs ++ kvs') m =
+  pupdates kvs' m ≫= pupdates kvs.
+Proof.
+  induction kvs as [|[k v] kvs IHkvs].
+  - cbn.
+    now destruct (pupdates kvs' m).
+  - cbn.
+    rewrite IHkvs.
+    now rewrite option_bind_assoc.
+Qed.
+
+Lemma extend_posmap_Piso_map kvs m m' :
+  pupdates kvs m = Some m' ->
+  extend_posmap kvs m.(Piso_map) = Some m'.(Piso_map).
+Proof.
+  revert m m'; induction kvs as [|[k v] kvs IHkvs]; intros m m';
+  [now intros [= <-]|].
+  rewrite extend_posmap_cons.
+  intros Heq.
+  apply (pupdates_perm _ (kvs ++ [(k, v)])) in Heq as Heq'; [|solve_Permutation].
+  rewrite pupdates_app in Heq'.
+  cbn in Heq'.
+  revert Heq'.
+  intros (m'' & Hupd & Hkvs)%bind_Some.
+  apply extend_posmap_one_Piso_map' in Hupd.
+  rewrite Hupd.
+  cbn.
+  now apply IHkvs.
+Qed.
+
+
+Fixpoint mayzip {A B} (l : list A) (l' : list B) : option (list (A * B)) :=
+  match l, l' with
+  | [], [] => Some []
+  | a :: l, b :: l' => ((a,b)::.) <$> mayzip l l'
+  | _, _ => None
+  end.
+
+Lemma mayzip_Some {A B} (l : list A) (l' : list B) ll :
+  mayzip l l' = Some ll <->
+  length l = length l' /\ ll = zip l l'.
+Proof.
+  revert l' ll; induction l as [|a l IHl]; intros [|b l'];
+  [cbn; clear; naive_solver|easy..|].
+  intros [|(a', b') ll]; [split; [|easy]; cbn; now destruct (mayzip _ _)|].
+  cbn.
+  rewrite fmap_Some.
+  setoid_rewrite IHl.
+  clear.
+  naive_solver.
+Qed.
+
+Lemma mayzip_is_Some {A B} (l : list A) (l' : list B) :
+  is_Some (mayzip l l') <-> length l = length l'.
+Proof.
+  unfold is_Some.
+  setoid_rewrite mayzip_Some.
+  naive_solver.
+Qed.
+
+Lemma mayzip_fmap_l {A B C} (f : A -> B) (l : list A) (l' : list C) :
+  mayzip (f <$> l) l' = (fmap (M:=list) (prod_map f id)) <$> mayzip l l'.
+Proof.
+  apply option_eq.
+  intros ll.
+  rewrite mayzip_Some.
+  rewrite length_fmap.
+  rewrite fmap_Some.
+  setoid_rewrite mayzip_Some.
+  rewrite zip_fmap_l.
+  naive_solver.
+Qed.
+
+Lemma mayzip_fmap_r {A B C} (f : B -> C) (l : list A) (l' : list B) :
+  mayzip l (f <$> l') = (fmap (M:=list) (prod_map id f)) <$> mayzip l l'.
+Proof.
+  apply option_eq.
+  intros ll.
+  rewrite mayzip_Some.
+  rewrite length_fmap.
+  rewrite fmap_Some.
+  setoid_rewrite mayzip_Some.
+  rewrite zip_fmap_r.
+  naive_solver.
+Qed.
