theories/GraphCore/SPHyperGraph.v
@@ -1,10 +1,14 @@
 Require Export Aux_pos TESyntax.
 From stdpp Require Export gmultiset list sorting fin_maps.
 From stdpp Require Export pmap gmap.
+Require Export HyperGraphAux.
 
 (* A strongly permutative hyper edge is an indicator for the edge type and the source and target vertices *)
 Notation SPHyperEdge T := (T * gmultiset positive)%type.
 (* A S[trongly]P[ermutative]HyperGraph representation where edges have a type T and the graph is represented as a map of positives to (edge_data, input_vertices, output_vertices) *)
+
+#[export] Instance SPHyperEdge_equiv `{Equiv T} : Equiv (SPHyperEdge T) :=
+  prod_relation (≡) (=).
 
 Record SPHyperGraph {T} := mk_sphg {
   (* The edges of the hypergraph *)
@@ -58,3 +62,87 @@ Definition vertices_sphg {T} (sphg : SPHyperGraph T) : Pset :=
   fun sphg sphg' =>
   reindex_sphg (bcons false) (relabel_sphg (bcons false) sphg) ∪
   reindex_sphg (bcons true) (relabel_sphg (bcons true) sphg').
+
+
+#[export] Instance sphypergraph_equiv `{Equiv T} : Equiv (SPHyperGraph T) :=
+  fun sphg sphg' =>
+  sphg.(sphyperedges) ≡ sphg'.(sphyperedges) /\
+  sphg.(sphypervertices) = sphg'.(sphypervertices).
+
+#[export] Instance sphypergraph_equivalence `{Equiv T, Equivalence T equiv} :
+  Equivalence (≡@{SPHyperGraph T}).
+Proof.
+  apply rel_intersection_equiv.
+  - refine (rel_preimage_equiv sphyperedges _ _).
+  - refine (rel_preimage_equiv sphypervertices _ _).
+Qed.
+
+
+Add Parametric Morphism `{Equiv T} : (@vertices_sphg T) with signature
+  (≡) ==> eq as vertices_sphg_equiv.
+Proof.
+  intros sphg sphg' [Heq Hverts].
+  unfold vertices_sphg.
+  rewrite <- Hverts.
+  f_equal.
+  apply map_to_list_equiv in Heq.
+  induction Heq as [|? ? ? ? Hhd]; [done|].
+  cbn.
+  rewrite 2 (list_to_set_app_L).
+  f_equal; [|done].
+  do 2 f_equal; apply Hhd.2.2.
+Qed.
+
+Add Parametric Morphism `{Equiv T} (f : positive -> positive) : 
+  (prod_map (@id T) (gmultiset_map f)) with signature
+  (≡) ==> (≡) as relabel_spabs_proper.
+Proof.
+  intros [t v] [t' v'] [? ?]; split; cbn; [done|now f_equal].
+Qed.
+
+Add Parametric Morphism `{Equiv T, Reflexive T equiv} f : (@relabel_sphg T f) with signature
+  (≡) ==> (≡) as relabel_sphg_proper.
+Proof.
+  intros sphg sphg' [Heq Hverts].
+  split; [|cbn; now f_equal].
+  cbn.
+  apply (map_fmap_proper _ _); [|done].
+  apply relabel_spabs_proper_Proper.
+Qed.
+
+Add Parametric Morphism `{Equiv T, Reflexive T equiv} f : (@reindex_sphg T f) with signature
+  (≡) ==> (≡) as reindex_sphg_proper.
+Proof.
+  intros sphg sphg' [Heq Hverts].
+  split; [|apply Hverts].
+  cbn.
+  now f_equiv.
+Qed.
+
+Add Parametric Morphism `{Equiv T} : (@union (SPHyperGraph T) _) with signature
+  (≡) ==> (≡) ==> (≡) as sphypergraph_union_proper.
+Proof.
+  intros sphg1 sphg1' Hsphg1 sphg2 sphg2' Hsphg2.
+  split; [|cbn; f_equal; [apply Hsphg1|apply Hsphg2]].
+  cbn.
+  apply union_proper; [apply Hsphg1|apply Hsphg2].
+Qed.
+
+
+Add Parametric Morphism `{Equiv T} : (@disj_union (SPHyperGraph T) _) with signature
+  (≡) ==> (≡) ==> (≡) as sphypergraph_disj_union_proper.
+Proof.
+  intros sphg1 sphg1' Hsphg1 sphg2 sphg2' Hsphg2.
+  split; [|cbn; do 2 f_equal; [apply Hsphg1|apply Hsphg2]].
+  cbn.
+  apply union_proper; f_equiv; 
+  (apply map_fmap_proper; [apply relabel_spabs_proper_Proper|]); 
+  [apply Hsphg1|apply Hsphg2].
+Qed.
+
+
+Lemma sphyperedges_singleton {T} k abs :
+  sphyperedges (T:=T) {[k := abs]} = {[k := abs]}.
+Proof.
+  done.
+Qed.
