theories/GraphCore/SPTensorGraphQuote.v
@@ -1,0 +1,674 @@
+Require Export SPTensorGraphHom AbstractTensorQuote SPIsomorphismTesting.
+
+(* TODO: Quote from CospanSPHyperGraph T to
+  CospanSPHyperGraph positive, via CospanSPHyperGraph (option T).
+  Prove can test for isomorphism in quoted. *)
+
+(* FIXME: Move *)
+Lemma spgraph_of_tensor_cosphg_eq `{Equiv T} (t t' : T) n m : t ≡ t' ->
+  cosphg_eq (spgraph_of_tensor t n m) (spgraph_of_tensor t' n m).
+Proof.
+  intros Ht.
+  apply mk_cosphg_eq; [done..|].
+  cbn.
+  split; [|done].
+  rewrite 2 sphyperedges_singleton.
+  rewrite <- insert_empty.
+  apply insert_proper; [|apply map_empty_equiv_eq; done].
+  split;[|done].
+  apply Ht.
+Qed.
+
+Add Parametric Morphism `{Equiv T, Equivalence T equiv}
+  {n m o} : (@compose_spgraphs_aux T n m o)
+  with signature cosphg_eq ==> cosphg_eq ==> cosphg_eq
+  as compose_spgraphs_aux_cosphg_eq.
+Proof.
+  intros cosphg1 cosphg1' (Hin1 & Hout1 & He1)
+    cosphg2 cosphg2' (Hin2 & Hout2 & He2).
+  unfold compose_spgraphs_aux.
+  rewrite <- Hin1, <- Hout1, <- Hin2, <- Hout2.
+  apply relabel_spgraph_cosphg_eq_Proper.
+  apply mk_cosphg_eq; [done..|].
+  cbn.
+  f_equiv.
+  now apply sphypergraph_union_proper.
+Qed.
+
+Add Parametric Morphism `{Equiv T, Equivalence T equiv}
+  {n m o} : (@compose_spgraphs T n m o)
+  with signature cosphg_eq ==> cosphg_eq ==> cosphg_eq
+  as compose_spgraphs_cosphg_eq.
+Proof.
+  intros cosphg1 cosphg1' Heq1
+    cosphg2 cosphg2' Heq2.
+  rewrite 2 compose_spgraphs_to_compose_spgraphs_aux.
+  now f_equiv; apply reindex_spgraph_cosphg_eq_Proper, 
+    relabel_spgraph_cosphg_eq_Proper.
+Qed.
+
+Add Parametric Morphism `{Equiv T, Equivalence T equiv}
+  {n m o} : (@compose_spgraphs_unsafe T n m o)
+  with signature cosphg_eq ==> cosphg_eq ==> cosphg_eq
+  as compose_spgraphs_unsafe_cosphg_eq.
+Proof.
+  intros cosphg1 cosphg1' (Hin1 & Hout1 & He1)
+    cosphg2 cosphg2' (Hin2 & Hout2 & He2).
+  unfold compose_spgraphs_unsafe.
+  rewrite <- Hin1, <- Hin2, <- Hout2.
+  apply mk_cosphg_eq; [done..|].
+  cbn.
+  f_equiv.
+  now apply sphypergraph_union_proper.
+Qed.
+
+Add Parametric Morphism `{Equiv T} {n m} : (@spreferrenced_vertices T n m)
+  with signature cosphg_eq ==> eq as spreferrenced_vertices_cosphg_eq.
+Proof.
+  intros cosphg cosphg' (Hins & Houts & [Heq Hverts]).
+  unfold spreferrenced_vertices.
+  rewrite <- Hins, Houts.
+  f_equal.
+  apply map_to_list_equiv in Heq.
+  induction Heq as [|? ? ? ? Hhd]; [done|].
+  cbn.
+  rewrite 2 (list_to_set_app_L).
+  f_equal; [|done].
+  do 2 f_equal; apply Hhd.
+Qed.
+
+Add Parametric Morphism `{Equiv T} {n m} : (@spisolated_vertices T n m)
+  with signature cosphg_eq ==> eq as spisolated_vertices_cosphg_eq.
+Proof.
+  intros cosphg cosphg' Heq.
+  unfold spisolated_vertices.
+  f_equal; [|now rewrite Heq].
+  apply Heq.2.2.2.
+Qed.
+
+Add Parametric Morphism `{Equiv T} {n m} : (@set_spverts T n m)
+  with signature cosphg_eq ==> eq ==> cosphg_eq as set_spverts_cosphg_eq.
+Proof.
+  intros cosphg cosphg' (Hins & Houts & [Heq Hverts]) vs.
+  apply mk_cosphg_eq; [done..|].
+  split; [done|].
+  done.
+Qed.
+
+
+Add Parametric Morphism `{Equiv T} {n m} : (@norm_spverts T n m)
+  with signature cosphg_eq ==> cosphg_eq as norm_spverts_cosphg_eq.
+Proof.
+  intros cosphg cosphg' Heq.
+  unfold norm_spverts.
+  now apply set_spverts_cosphg_eq, spisolated_vertices_cosphg_eq_Proper.
+Qed.
+
+
+
+
+
+
+
+
+Class CospanSPHyperGraphQuote {Ctx T} `{Equiv T'} (f : Ctx -> T -> T')
+  (ctx : Ctx) {n m} (expr : CospanSPHyperGraph T n m) (val : CospanSPHyperGraph T' n m) := {
+  cosphg_quote : cosphg_eq (spgraph_apply_hom (f ctx) expr) val;
+}.
+
+#[global] Hint Mode CospanSPHyperGraphQuote + + + - + - + + - + : typeclass_instances.
+
+
+Lemma cosphg_quote_correct_equiv {Ctx} `{Equiv T, Equivalence T equiv,
+  Equiv T', Equivalence T' equiv}
+  (f : Ctx -> T -> T')
+  (ctx : Ctx) {n m} (expr expr' : CospanSPHyperGraph T n m)
+    (val val' : CospanSPHyperGraph T' n m)
+    {Hval : CospanSPHyperGraphQuote f ctx expr val}
+    {Hval' : CospanSPHyperGraphQuote f ctx expr' val'}
+    {Hf : Proper (equiv ==> equiv) (f ctx)} :
+  expr ≡ expr' -> val ≡ val'.
+Proof.
+  intros Heq.
+  destruct Hval as [Hval].
+  destruct Hval' as [Hval'].
+  rewrite <- Hval.
+  etransitivity; [|apply cosphg_eq_subrelation, Hval'].
+  refine (spgraph_apply_hom_proper_Proper _ _ _ _ _).
+  done.
+Qed.
+
+
+Section instances.
+
+#[local] Set Typeclasses Unique Instances.
+
+Context {Ctx T} `{Equiv T'} `{Equivalence T' equiv} (f : Ctx -> T -> T')
+  (ctx : Ctx).
+
+Local Notation Quote := (@CospanSPHyperGraphQuote Ctx T T' _ f ctx _ _).
+
+#[export] Instance cosphg_quote_spgraph_apply_hom {n m} (expr : CospanSPHyperGraph T n m) :
+  Quote expr (spgraph_apply_hom (f ctx) expr).
+Proof.
+  now constructor.
+Qed.
+
+#[export] Instance cosphg_quote_id_spgraph {n} : Quote (id_spgraph n) (id_spgraph n).
+Proof.
+  constructor.
+  done.
+Qed.
+
+#[export] Instance cosphg_quote_cup_spgraph {n} : Quote (cup_spgraph n) (cup_spgraph n).
+Proof.
+  constructor.
+  done.
+Qed.
+
+#[export] Instance cosphg_quote_cap_spgraph {n} : Quote (cap_spgraph n) (cap_spgraph n).
+Proof.
+  constructor.
+  done.
+Qed.
+
+#[export] Instance cosphg_quote_swap_spgraph {n m} : Quote (swap_spgraph n m) (swap_spgraph n m).
+Proof.
+  constructor.
+  done.
+Qed.
+
+#[export] Instance cosphg_quote_spgraph_of_tensor {n m} t t' :
+  AbstractTensorQuote f ctx t t' ->
+  Quote (spgraph_of_tensor t n m) (spgraph_of_tensor t' n m).
+Proof.
+  intros [Ht].
+  constructor.
+  rewrite spgraph_apply_hom_spgraph_of_tensor.
+  now apply spgraph_of_tensor_cosphg_eq.
+Qed.
+
+Lemma quote_of_unary_mor {n m n' m'}
+  (g : forall T'', CospanSPHyperGraph T'' n m -> CospanSPHyperGraph T'' n' m')
+  (Hg : Proper (cosphg_eq ==> cosphg_eq) (g T'))
+  (Hghom : forall cosphg, spgraph_apply_hom (f ctx) (g T cosphg) =
+      g T' (spgraph_apply_hom (f ctx) cosphg)) :
+  forall expr val, Quote expr val -> Quote (g T expr) (g T' val).
+Proof.
+  intros expr val [Hval].
+  constructor.
+  rewrite Hghom.
+  now apply Hg.
+Qed.
+
+Lemma quote_of_binary_mor {n m n' m' n'' m''}
+  (g : forall T'', CospanSPHyperGraph T'' n m -> CospanSPHyperGraph T'' n' m' ->
+    CospanSPHyperGraph T'' n'' m'')
+  (Hg : Proper (cosphg_eq ==> cosphg_eq ==> cosphg_eq) (g T'))
+  (Hghom : forall cosphg cosphg', spgraph_apply_hom (f ctx) (g T cosphg cosphg') =
+      g T' (spgraph_apply_hom (f ctx) cosphg) (spgraph_apply_hom (f ctx) cosphg')) :
+  forall expr expr' val val', Quote expr val -> Quote expr' val' ->
+    Quote (g T expr expr') (g T' val val').
+Proof.
+  intros expr expr' val val' [Hval] [Hval'].
+  constructor.
+  rewrite Hghom.
+  now apply Hg.
+Qed.
+
+#[export] Instance cosphg_quote_relabel_spgraph {n m}
+  g (expr : CospanSPHyperGraph T n m) val :
+  Quote expr val ->
+  Quote (relabel_spgraph g expr)
+    (relabel_spgraph g val).
+Proof.
+  apply (quote_of_unary_mor (fun _ => _) _).
+  intros; apply spgraph_apply_hom_relabel_spgraph.
+Qed.
+
+#[export] Instance cosphg_quote_reindex_spgraph {n m}
+  g (expr : CospanSPHyperGraph T n m) val :
+  Quote expr val ->
+  Quote (reindex_spgraph g expr)
+    (reindex_spgraph g val).
+Proof.
+  apply (quote_of_unary_mor (fun _ => _) _).
+  intros; apply spgraph_apply_hom_reindex_spgraph.
+Qed.
+
+#[export] Instance cosphg_quote_swapped_stack_spgraphs_aux {n m n' m'}
+  (expr : CospanSPHyperGraph T n m) (expr' : CospanSPHyperGraph T n' m')
+  val val' :
+  Quote expr val -> Quote expr' val' ->
+  Quote (swapped_stack_spgraphs_aux expr expr')
+    (swapped_stack_spgraphs_aux val val').
+Proof.
+  apply (quote_of_binary_mor (fun _ => _) _).
+  intros; apply spgraph_apply_hom_swapped_stack_spgraphs_aux.
+Qed.
+
+#[export] Instance cosphg_quote_swapped_stack_spgraphs {n m n' m'}
+  (expr : CospanSPHyperGraph T n m) (expr' : CospanSPHyperGraph T n' m')
+  val val' :
+  Quote expr val -> Quote expr' val' ->
+  Quote (swapped_stack_spgraphs expr expr')
+    (swapped_stack_spgraphs val val').
+Proof.
+  apply (quote_of_binary_mor (fun _ => _) _).
+  intros; apply spgraph_apply_hom_swapped_stack_spgraphs.
+Qed.
+
+#[export] Instance cosphg_quote_stack_spgraphs_aux {n m n' m'}
+  (expr : CospanSPHyperGraph T n m) (expr' : CospanSPHyperGraph T n' m')
+  val val' :
+  Quote expr val -> Quote expr' val' ->
+  Quote (stack_spgraphs_aux expr expr')
+    (stack_spgraphs_aux val val').
+Proof.
+  apply (quote_of_binary_mor (fun _ => _) _).
+  intros; apply spgraph_apply_hom_stack_spgraphs_aux.
+Qed.
+
+#[export] Instance cosphg_quote_stack_spgraphs {n m n' m'}
+  (expr : CospanSPHyperGraph T n m) (expr' : CospanSPHyperGraph T n' m')
+  val val' :
+  Quote expr val -> Quote expr' val' ->
+  Quote (stack_spgraphs expr expr')
+    (stack_spgraphs val val').
+Proof.
+  apply (quote_of_binary_mor (fun _ => _) _).
+  intros; apply spgraph_apply_hom_stack_spgraphs.
+Qed.
+
+#[export] Instance cosphg_quote_spadd_top_loop {n m}
+  (expr : CospanSPHyperGraph T (S n) (S m)) val :
+  Quote expr val ->
+  Quote (spadd_top_loop expr)
+    (spadd_top_loop val).
+Proof.
+  apply (quote_of_unary_mor (fun _ => _) _).
+  intros; apply spgraph_apply_hom_spadd_top_loop.
+Qed.
+
+#[export] Instance cosphg_quote_spadd_top_loops {n m o}
+  (expr : CospanSPHyperGraph T (n + m) (n + o)) val :
+  Quote expr val ->
+  Quote (spadd_top_loops expr)
+    (spadd_top_loops val).
+Proof.
+  apply (quote_of_unary_mor (fun _ => _) _).
+  intros; apply spgraph_apply_hom_spadd_top_loops.
+Qed.
+
+#[export] Instance cosphg_quote_compose_spgraphs_aux {n m o}
+  (expr : CospanSPHyperGraph T n m) (expr' : CospanSPHyperGraph T m o)
+  val val' :
+  Quote expr val -> Quote expr' val' ->
+  Quote (compose_spgraphs_aux expr expr')
+    (compose_spgraphs_aux val val').
+Proof.
+  apply (quote_of_binary_mor (fun _ => _) _).
+  intros; apply spgraph_apply_hom_compose_spgraphs_aux.
+Qed.
+
+#[export] Instance cosphg_quote_compose_spgraphs {n m o}
+  (expr : CospanSPHyperGraph T n m) (expr' : CospanSPHyperGraph T m o)
+  val val' :
+  Quote expr val -> Quote expr' val' ->
+  Quote (compose_spgraphs expr expr')
+    (compose_spgraphs val val').
+Proof.
+  apply (quote_of_binary_mor (fun _ => _) _).
+  intros; apply spgraph_apply_hom_compose_spgraphs.
+Qed.
+
+#[export] Instance cosphg_quote_compose_spgraphs_unsafe {n m o}
+  (expr : CospanSPHyperGraph T n m) (expr' : CospanSPHyperGraph T m o)
+  val val' :
+  Quote expr val -> Quote expr' val' ->
+  Quote (compose_spgraphs_unsafe expr expr')
+    (compose_spgraphs_unsafe val val').
+Proof.
+  apply (quote_of_binary_mor (fun _ => _) _).
+  intros; apply spgraph_apply_hom_compose_spgraphs_unsafe.
+Qed.
+
+#[export] Instance cosphg_quote_norm_spverts {n m}
+  (expr : CospanSPHyperGraph T n m) val :
+  Quote expr val ->
+  Quote (norm_spverts expr)
+    (norm_spverts val).
+Proof.
+  apply (quote_of_unary_mor (fun _ => _) _).
+  intros; apply spgraph_apply_hom_norm_spverts.
+Qed.
+
+End instances.
+
+
+
+
+Class CospanSPHyperGraphDenote {Ctx T} `{Equiv T'} (f : Ctx -> T -> T')
+  (ctx : Ctx) {n m} (expr : CospanSPHyperGraph T n m) (val : CospanSPHyperGraph T' n m) := {
+  cosphg_denote : cosphg_eq (spgraph_apply_hom (f ctx) expr) val;
+}.
+
+#[global] Hint Mode CospanSPHyperGraphDenote + + + - + - + + + - : typeclass_instances.
+
+Class AbstractTensorDenote {Ctx T} `{Equiv T'} (f : Ctx -> T -> T') (ctx : Ctx)
+  (t : T) (t' : T') := {
+  abs_denote : f ctx t ≡ t'
+}.
+
+#[global] Hint Mode AbstractTensorDenote + + + - + + + - : typeclass_instances.
+
+#[export] Instance abstens_denote_default {Ctx T} `{Equiv T', Reflexive T' equiv}
+  (f : Ctx -> T -> T') (ctx : Ctx) (t : T) :
+  AbstractTensorDenote f ctx t (f ctx t) | 100.
+Proof.
+  constructor.
+  reflexivity.
+Qed.
+
+
+Lemma cosphg_denote_correct_equiv {Ctx} `{Equiv T, Equivalence T equiv,
+  Equiv T', Equivalence T' equiv}
+  (f : Ctx -> T -> T')
+  (ctx : Ctx) {n m} (expr expr' : CospanSPHyperGraph T n m)
+    (val val' : CospanSPHyperGraph T' n m)
+    {Hval : CospanSPHyperGraphDenote f ctx expr val}
+    {Hval' : CospanSPHyperGraphDenote f ctx expr' val'}
+    {Hf : Proper (equiv ==> equiv) (f ctx)} :
+  expr ≡ expr' -> val ≡ val'.
+Proof.
+  intros Heq.
+  destruct Hval as [Hval].
+  destruct Hval' as [Hval'].
+  rewrite <- Hval.
+  etransitivity; [|apply cosphg_eq_subrelation, Hval'].
+  refine (spgraph_apply_hom_proper_Proper _ _ _ _ _).
+  done.
+Qed.
+
+Section instances.
+
+#[local] Set Typeclasses Unique Instances.
+
+Context {Ctx T} `{Equiv T'} `{Equivalence T' equiv} (f : Ctx -> T -> T')
+  (ctx : Ctx).
+
+Local Notation Denote := (@CospanSPHyperGraphDenote Ctx T T' _ f ctx _ _).
+
+#[export] Instance cosphg_denote_id_spgraph {n} : Denote (id_spgraph n) (id_spgraph n).
+Proof.
+  constructor.
+  done.
+Qed.
+
+#[export] Instance cosphg_denote_cup_spgraph {n} : Denote (cup_spgraph n) (cup_spgraph n).
+Proof.
+  constructor.
+  done.
+Qed.
+
+#[export] Instance cosphg_denote_cap_spgraph {n} : Denote (cap_spgraph n) (cap_spgraph n).
+Proof.
+  constructor.
+  done.
+Qed.
+
+#[export] Instance cosphg_denote_swap_spgraph {n m} : Denote (swap_spgraph n m) (swap_spgraph n m).
+Proof.
+  constructor.
+  done.
+Qed.
+
+#[export] Instance cosphg_denote_spgraph_of_tensor {n m} t t' :
+  AbstractTensorDenote f ctx t t' ->
+  Denote (spgraph_of_tensor t n m) (spgraph_of_tensor t' n m).
+Proof.
+  intros [Ht].
+  constructor.
+  rewrite spgraph_apply_hom_spgraph_of_tensor.
+  now apply spgraph_of_tensor_cosphg_eq.
+Qed.
+
+Lemma denote_of_unary_mor {n m n' m'}
+  (g : forall T'', CospanSPHyperGraph T'' n m -> CospanSPHyperGraph T'' n' m')
+  (Hg : Proper (cosphg_eq ==> cosphg_eq) (g T'))
+  (Hghom : forall cosphg, spgraph_apply_hom (f ctx) (g T cosphg) =
+      g T' (spgraph_apply_hom (f ctx) cosphg)) :
+  forall expr val, Denote expr val -> Denote (g T expr) (g T' val).
+Proof.
+  intros expr val [Hval].
+  constructor.
+  rewrite Hghom.
+  now apply Hg.
+Qed.
+
+Lemma denote_of_binary_mor {n m n' m' n'' m''}
+  (g : forall T'', CospanSPHyperGraph T'' n m -> CospanSPHyperGraph T'' n' m' ->
+    CospanSPHyperGraph T'' n'' m'')
+  (Hg : Proper (cosphg_eq ==> cosphg_eq ==> cosphg_eq) (g T'))
+  (Hghom : forall cosphg cosphg', spgraph_apply_hom (f ctx) (g T cosphg cosphg') =
+      g T' (spgraph_apply_hom (f ctx) cosphg) (spgraph_apply_hom (f ctx) cosphg')) :
+  forall expr expr' val val', Denote expr val -> Denote expr' val' ->
+    Denote (g T expr expr') (g T' val val').
+Proof.
+  intros expr expr' val val' [Hval] [Hval'].
+  constructor.
+  rewrite Hghom.
+  now apply Hg.
+Qed.
+
+#[export] Instance cosphg_denote_relabel_spgraph {n m}
+  g (expr : CospanSPHyperGraph T n m) val :
+  Denote expr val ->
+  Denote (relabel_spgraph g expr)
+    (relabel_spgraph g val).
+Proof.
+  apply (denote_of_unary_mor (fun _ => _) _).
+  intros; apply spgraph_apply_hom_relabel_spgraph.
+Qed.
+
+#[export] Instance cosphg_denote_reindex_spgraph {n m}
+  g (expr : CospanSPHyperGraph T n m) val :
+  Denote expr val ->
+  Denote (reindex_spgraph g expr)
+    (reindex_spgraph g val).
+Proof.
+  apply (denote_of_unary_mor (fun _ => _) _).
+  intros; apply spgraph_apply_hom_reindex_spgraph.
+Qed.
+
+#[export] Instance cosphg_denote_swapped_stack_spgraphs_aux {n m n' m'}
+  (expr : CospanSPHyperGraph T n m) (expr' : CospanSPHyperGraph T n' m')
+  val val' :
+  Denote expr val -> Denote expr' val' ->
+  Denote (swapped_stack_spgraphs_aux expr expr')
+    (swapped_stack_spgraphs_aux val val').
+Proof.
+  apply (denote_of_binary_mor (fun _ => _) _).
+  intros; apply spgraph_apply_hom_swapped_stack_spgraphs_aux.
+Qed.
+
+#[export] Instance cosphg_denote_swapped_stack_spgraphs {n m n' m'}
+  (expr : CospanSPHyperGraph T n m) (expr' : CospanSPHyperGraph T n' m')
+  val val' :
+  Denote expr val -> Denote expr' val' ->
+  Denote (swapped_stack_spgraphs expr expr')
+    (swapped_stack_spgraphs val val').
+Proof.
+  apply (denote_of_binary_mor (fun _ => _) _).
+  intros; apply spgraph_apply_hom_swapped_stack_spgraphs.
+Qed.
+
+#[export] Instance cosphg_denote_stack_spgraphs_aux {n m n' m'}
+  (expr : CospanSPHyperGraph T n m) (expr' : CospanSPHyperGraph T n' m')
+  val val' :
+  Denote expr val -> Denote expr' val' ->
+  Denote (stack_spgraphs_aux expr expr')
+    (stack_spgraphs_aux val val').
+Proof.
+  apply (denote_of_binary_mor (fun _ => _) _).
+  intros; apply spgraph_apply_hom_stack_spgraphs_aux.
+Qed.
+
+#[export] Instance cosphg_denote_stack_spgraphs {n m n' m'}
+  (expr : CospanSPHyperGraph T n m) (expr' : CospanSPHyperGraph T n' m')
+  val val' :
+  Denote expr val -> Denote expr' val' ->
+  Denote (stack_spgraphs expr expr')
+    (stack_spgraphs val val').
+Proof.
+  apply (denote_of_binary_mor (fun _ => _) _).
+  intros; apply spgraph_apply_hom_stack_spgraphs.
+Qed.
+
+#[export] Instance cosphg_denote_spadd_top_loop {n m}
+  (expr : CospanSPHyperGraph T (S n) (S m)) val :
+  Denote expr val ->
+  Denote (spadd_top_loop expr)
+    (spadd_top_loop val).
+Proof.
+  apply (denote_of_unary_mor (fun _ => _) _).
+  intros; apply spgraph_apply_hom_spadd_top_loop.
+Qed.
+
+#[export] Instance cosphg_denote_spadd_top_loops {n m o}
+  (expr : CospanSPHyperGraph T (n + m) (n + o)) val :
+  Denote expr val ->
+  Denote (spadd_top_loops expr)
+    (spadd_top_loops val).
+Proof.
+  apply (denote_of_unary_mor (fun _ => _) _).
+  intros; apply spgraph_apply_hom_spadd_top_loops.
+Qed.
+
+#[export] Instance cosphg_denote_compose_spgraphs_aux {n m o}
+  (expr : CospanSPHyperGraph T n m) (expr' : CospanSPHyperGraph T m o)
+  val val' :
+  Denote expr val -> Denote expr' val' ->
+  Denote (compose_spgraphs_aux expr expr')
+    (compose_spgraphs_aux val val').
+Proof.
+  apply (denote_of_binary_mor (fun _ => _) _).
+  intros; apply spgraph_apply_hom_compose_spgraphs_aux.
+Qed.
+
+#[export] Instance cosphg_denote_compose_spgraphs {n m o}
+  (expr : CospanSPHyperGraph T n m) (expr' : CospanSPHyperGraph T m o)
+  val val' :
+  Denote expr val -> Denote expr' val' ->
+  Denote (compose_spgraphs expr expr')
+    (compose_spgraphs val val').
+Proof.
+  apply (denote_of_binary_mor (fun _ => _) _).
+  intros; apply spgraph_apply_hom_compose_spgraphs.
+Qed.
+
+#[export] Instance cosphg_denote_compose_spgraphs_unsafe {n m o}
+  (expr : CospanSPHyperGraph T n m) (expr' : CospanSPHyperGraph T m o)
+  val val' :
+  Denote expr val -> Denote expr' val' ->
+  Denote (compose_spgraphs_unsafe expr expr')
+    (compose_spgraphs_unsafe val val').
+Proof.
+  apply (denote_of_binary_mor (fun _ => _) _).
+  intros; apply spgraph_apply_hom_compose_spgraphs_unsafe.
+Qed.
+
+#[export] Instance cosphg_denote_norm_spverts {n m}
+  (expr : CospanSPHyperGraph T n m) val :
+  Denote expr val ->
+  Denote (norm_spverts expr)
+    (norm_spverts val).
+Proof.
+  apply (denote_of_unary_mor (fun _ => _) _).
+  intros; apply spgraph_apply_hom_norm_spverts.
+Qed.
+
+End instances.
+
+
+
+
+
+
+#[local] Program Instance opttensor_TensorLike
+  `{TensorLike R rO rI radd rmul req A T} : TensorLike R A (option T) := {
+  interpretTensor mt := from_option interpretTensor (fun _ _ => const_tensor rO) mt;
+}.
+Next Obligation.
+  intros *.
+  intros mt mt' Hmt.
+  induction Hmt as [mt mt' Hmt|]; [|done].
+  cbn.
+  now apply interpretTensorProper.
+Qed.
+
+#[export] Instance Some_TensorProper `{Equiv T} :
+  Proper (equiv ==> equiv) (@Some T) :=
+  Some_proper.
+
+#[export] Instance Some_TensorLikeHom `{TensorLike R rO rI radd rmul req A T} :
+  TensorLikeHom R A (@Some T).
+Proof.
+  split.
+  reflexivity.
+Qed.
+
+
+
+Lemma spgraph_to_option_correct_equiv `{Equiv T, Equivalence T equiv}
+  {n m} (expr expr' : CospanSPHyperGraph T n m) val val' :
+  CospanSPHyperGraphDenote (fun _ => Some) tt expr val ->
+  CospanSPHyperGraphDenote (fun _ => Some) tt expr' val' ->
+  val ≡ val' ->
+  expr ≡ expr'.
+Proof.
+  intros [Hval] [Hval'] Heq.
+  rewrite <- Hval, <- Hval' in Heq.
+  now apply (spgraph_apply_hom_equiv_inv Some).
+Qed.
+
+
+
+Local Existing Instance positive_equiv.
+
+
+Lemma spgraph_equiv_of_positive `{Equiv T, Equivalence T equiv}
+  (ctx : list T) {n m} (expr expr' : CospanSPHyperGraph positive n m) 
+  val val' oval oval' :
+  CospanSPHyperGraphDenote (λ _, Some) tt val oval ->
+  CospanSPHyperGraphDenote (λ _, Some) tt val' oval' ->
+  CospanSPHyperGraphQuote interp_discrete_hg ctx expr oval ->
+  CospanSPHyperGraphQuote interp_discrete_hg ctx expr' oval' ->
+  expr ≡ expr' ->
+  val ≡ val'.
+Proof.
+  intros Hoval Hoval' Hval Hval'.
+  intros Heq.
+  apply (cosphg_quote_correct_equiv interp_discrete_hg ctx _ _ oval oval') in Heq.
+  revert Heq.
+  apply spgraph_to_option_correct_equiv; apply _.
+Qed.
+
+Lemma spgraph_test_isomorphism_quote `{Equiv T, Equivalence T equiv}
+  (ctx : list T) {n m} (expr expr' : CospanSPHyperGraph positive n m) val val' oval oval' :
+  CospanSPHyperGraphDenote (λ _, Some) tt val oval ->
+  CospanSPHyperGraphDenote (λ _, Some) tt val' oval' ->
+  CospanSPHyperGraphQuote interp_discrete_hg ctx expr oval ->
+  CospanSPHyperGraphQuote interp_discrete_hg ctx expr' oval' ->
+  spgraph_iso_partial_test expr expr' = true ->
+  norm_spverts val ≡ norm_spverts val'.
+Proof.
+  intros Hoval Hoval' Hval Hval' Heq%spgraph_iso_partial_test_correct.
+  revert Heq.
+  apply spgraph_equiv_of_positive with ctx (norm_spverts oval) (norm_spverts oval');
+    apply _.
+Qed.
+
+
+
+
